theories/rules/poll.v
@@ -8,24 +8,28 @@ Section poll.
 
 Context `{vmG: !gen_VMG Σ}.
   
-Lemma poll {w1 r0 q p s E rxp l j} ai i :
+Lemma poll {w1 r0 q p s E rxp l j r1 r2} ai i :
   decode_instruction w1 = Some Hvc ->
   decode_hvc_func r0 = Some Poll ->
   addr_in_page ai p ->
   p ∈ s ->
   {SS{{ ▷ (PC @@ i ->r ai)
           ∗ ▷ (R0 @@ i ->r r0)
+          ∗ ▷ (R1 @@ i ->r r1)
+          ∗ ▷ (R2 @@ i ->r r2)
           ∗ ▷ (ai ->a w1)
           ∗ ▷ (A@i :={q}[s] )
           ∗ ▷ (RX@ i :=( rxp ! l, j))}}}
     ExecI @ i ;E
     {{{ RET ExecI; PC @@ i ->r (ai ^+ 1)%f
-                     ∗ R0 @@ i ->r r0
+                     ∗ R0 @@ i ->r (encode_hvc_func Send)
+                     ∗ R1 @@ i ->r l
+                     ∗ R2 @@ i ->r (encode_vmid j)             
                      ∗ ai ->a w1
                      ∗ A@i :={q}[s]
                      ∗ RX@ i :=( rxp !)}}}.
 Proof.
-  iIntros (Hdecinstr Hdechvc Haddr Hins ϕ) "(>HPC & >HR0 & >Hai & >Hacc & >Hrx) Hϕ".
+  iIntros (Hdecinstr Hdechvc Haddr Hins ϕ) "(>HPC & >HR0 & >HR1 & >HR2 & >Hai & >Hacc & >Hrx) Hϕ".
   iApply (sswp_lift_atomic_step ExecI); [done|].
   iIntros (σ1) "%Hsche Hσ".
   inversion Hsche as [ Hcur ]; clear Hsche.
@@ -35,6 +39,8 @@ Proof.
   (* valid regs *)
   iDestruct (gen_reg_valid1 PC i ai Hcur with "Hregown HPC") as "%HPC".
   iDestruct (gen_reg_valid1 R0 i r0 Hcur with "Hregown HR0") as "%HR0".
+  iDestruct (gen_reg_valid1 R1 i r1 Hcur with "Hregown HR1") as "%HR1".
+  iDestruct (gen_reg_valid1 R2 i r2 Hcur with "Hregown HR2") as "%HR2".
   (* valid pt *)
   iDestruct (gen_access_valid_addr_Set ai p s with "Haccessown Hacc") as %Hacc; eauto.
   (* valid mem *)
@@ -53,6 +59,7 @@ Proof.
     rewrite  HR0 Hdechvc /poll in Heqc2.
     rewrite /is_rx_ready in Heqc2.
     rewrite /is_rx_ready_global in Heqc2.
+    rewrite /get_rx_length /get_rx_sender /get_rx_length_global /get_rx_sender_global in Heqc2.
     destruct (get_vm_mail_box σ1 (get_current_vm σ1)) as [tx rx] eqn:Heqmb.
     destruct rx as [rxaddr rxstatus] eqn:Heqrx.
     rewrite Hcur in Heqmb.
@@ -67,42 +74,66 @@ Proof.
     simpl.
     rewrite /gen_vm_interp /update_incr_PC.
     rewrite_reg_pc.
+    rewrite /update_reg.
+    do 3 rewrite_reg_global.
     rewrite /empty_rx.
     rewrite_empty_rx_global.
     iFrame "Hrest Htx Hrx1 Hmemown Haccessown Hown Htokown".
-    iDestruct ((gen_reg_update1_global PC (get_current_vm σ1) ai (ai ^+ 1)%f) with "Hregown HPC") as "HpcUpd".
-    rewrite ->(update_offset_PC_update_PC1 _ (get_current_vm σ1) ai 1); auto.
-    2 : {
-      by rewrite empty_rx_global_preserve_current_vm.
-    }
-    2 : {
-      apply get_reg_gmap_get_reg_Some; auto.
-      by rewrite empty_rx_global_preserve_current_vm.
-      rewrite /empty_rx_global.
-      rewrite /get_current_vm.
-      rewrite (surjective_pairing (get_vm_mail_box σ1 σ1.1.1.2)).
-      rewrite (surjective_pairing (get_vm_mail_box σ1 σ1.1.1.2).2).
-      rewrite /get_reg.
-      rewrite /get_reg_global.
-      rewrite /get_vm_reg_file.
-      rewrite /get_reg_files.
-      simpl.
-      rewrite /get_current_vm.
-      simpl.
-      by rewrite /get_reg /get_reg_global /get_current_vm /get_vm_reg_file /get_reg_files in HPC.
-    }
-    iMod "HpcUpd".
+    iDestruct ((gen_reg_update4_global PC (get_current_vm σ1) (ai ^+ 1)%f
+                                       R2 (get_current_vm σ1) (encode_vmid j)
+                                       R1 (get_current_vm σ1) l
+                                       R0 (get_current_vm σ1) (encode_hvc_func Send))
+                 with "Hregown HPC HR2 HR1 HR0") as ">[Hregown [PC [R2 [R1 R0]]]]"; eauto.
+    rewrite ->(update_offset_PC_update_PC1 _ (get_current_vm σ1) ai 1).
+    rewrite !update_reg_global_update_reg.
+    rewrite empty_rx_global_preserve_regs.
+    iFrame.
     iDestruct (gen_rx_gmap_update_empty_global_Some (get_current_vm σ1) rxp with "Hrx2 Hrx") as "Hrx'".
     iMod "Hrx'".
     iDestruct "Hrx'" as "[? ?]".
     iModIntro.
-    iDestruct "HpcUpd" as "[? ?]".
-    rewrite empty_rx_global_preserve_regs.
-    iFrame.
     rewrite empty_rx_global_update_mailbox.
     iFrame.
     iApply "Hϕ".
     by iFrame.
+    exists r0.
+    rewrite empty_rx_global_preserve_regs.
+    apply get_reg_gmap_get_reg_Some; auto.
+    exists r1.
+    rewrite lookup_insert_ne; [|done].
+    rewrite empty_rx_global_preserve_regs.
+    apply get_reg_gmap_get_reg_Some; auto.
+    exists r0.
+    rewrite empty_rx_global_preserve_regs.
+    apply get_reg_gmap_get_reg_Some; auto.
+    exists r2.
+    do 2 (rewrite lookup_insert_ne; [|done]).
+    rewrite empty_rx_global_preserve_regs.    
+    apply get_reg_gmap_get_reg_Some; auto.
+    exists r0.
+    rewrite empty_rx_global_preserve_regs.
+    apply get_reg_gmap_get_reg_Some; auto.
+    exists r1.
+    rewrite lookup_insert_ne; [|done].
+    rewrite empty_rx_global_preserve_regs.
+    apply get_reg_gmap_get_reg_Some; auto.
+    exists r0.
+    rewrite empty_rx_global_preserve_regs.
+    apply get_reg_gmap_get_reg_Some; auto.
+    by rewrite !update_reg_global_preserve_current_vm empty_rx_global_preserve_current_vm.
+    rewrite !update_reg_global_update_reg empty_rx_global_preserve_regs;try solve_reg_lookup.
+    do 3 (rewrite lookup_insert_ne; [|done]).
+    apply get_reg_gmap_get_reg_Some; auto.
+    exists r1.
+    rewrite lookup_insert_ne.
+    solve_reg_lookup.
+    done.
+    exists r2.
+    do 2 (rewrite lookup_insert_ne; [|done]).
+    solve_reg_lookup.
+    exists r1.
+    rewrite lookup_insert_ne; [|done].
+    solve_reg_lookup.
 Qed.
 
 End poll.
